Add files via upload

A1/Q3.dfy
@@ -1,9 +1,21 @@
+function method findSum(sum : nat, next: nat, i : nat): (nat, nat)
+requires i >= 0;
+requires sum >= 0 && sum <= i;
+requires next >= 0;
+decreases i - sum - next
+ensures sum <= i;
+{
+    //var x := i - sum;
+    //var y := next - x - 1;
+    if (sum + next <= i) then findSum(sum + next, next + 1, i) else (i - sum, next - (i - sum) - 1)
+}
+
 function method unpair (i: nat ): (nat, nat)
 requires i >= 0;
-decreases i;
-{ 
-    if (i == 0) then (0, 0) else var (p, q) := unpair(i - 1); 
-    if (q > 0) then (p + 1, q - 1) else (q, p + 1)
+{ // TODO 
+    var (x, y) := findSum(0, 0, i);
+    var part := (x,y);
+    part
 }
 
 function method pick (i: nat ): nat
@@ -12,36 +24,29 @@ function method pick (i: nat ): nat
     x + i * y
 }
 
-function method reverse (x: nat, y: nat): nat
-    decreases x + y, x
-{
-    if (x == 0 && y == 0) then 0 else
-        if (x > 0 && y >= 0) then 1 + reverse(x - 1, y + 1) else
-            if (x == 0 && y > 0) then 1 + reverse(y - 1, x) else 
-                0
-}
-
-lemma check(a: nat , b: nat, i: nat)
-    requires a >= 0;
-    requires b >= 0;
-    requires i >= 0;
-    ensures reverse(a, b) >= i;
-    ensures exists x, y :: i == reverse(x, y) == reverse(a, b) ==> x == unpair(i).0 && y == unpair(i).1;
-{
-
-}
-
 method catchTheSpy (a: nat , b: nat )
 {
     var i := 0;
     while a + i * b != pick (i)
-    invariant reverse(a, b) >= 0;
-    decreases reverse(a, b) - i; 
+   // assert (a + b) >= findXYSum(i));
+   // invariant (findXYSum(i) == findXYSum(i+1) || findXYSum(i) + 1 == findXYSum(i+1));
+    decreases ((a + b) - findXYSum(i)), findY(i); 
     { 
-        check(a, b, i);
+        //
         i := i + 1; 
     }
+    
 }
 
+function method findXYSum(i: nat): nat
+{
+    var (x, y) := unpair (i);
+    x + y
+}
 
-
+function method findY(i: nat): nat
+{
+    var (x, y) := unpair (i);
+    y
+}
+// a + i * b == x + i * y
